attempts on hash table

pulse/share/steel/examples/pulse/dice/lib/PulseHashTable.fst
@@ -32,6 +32,37 @@ let coerce_us (n:nat) : US.t = assume (US.fits n); US.uint_to_t n
   See FIXME comments for current debugging status
 *)
 #set-options "--split_queries no"
+
+let insert_loop_inv_def (#s:pht_sig) (b:bool)
+  (pht:(p:pht s{not_full p.repr}))
+  (ht:ht s)
+  (off: R.ref nat) (cont: R.ref bool)
+  (k:s.keyt) (v:s.valt)
+  (voff:nat) (vcont:bool)
+=
+  // `@(if vcont=true 
+  //   then (A.pts_to ht.contents full_perm pht.repr) 
+  //   else (A.pts_to ht.contents full_perm (PHT.insert pht k v).repr)) `star`
+  R.pts_to off full_perm voff `star`
+  R.pts_to cont full_perm vcont `star`
+  models s (if vcont then pht else PHT.insert pht k v) ht `star`
+  pure (
+    voff >= 0 /\ voff <= ht.sz /\
+    // walk_ pht.repr cidx k off == PHT.insert pht k v /\
+    // walk pht.repr cidx k off == lookup_repr pht.repr k /\
+    // strong_all_used_not_by #s #sz pht.repr cidx voff k /\
+    b == (voff <= ht.sz && vcont = true))
+
+let insert_loop_inv (#s:pht_sig) (b:bool)
+  (pht:(p:pht s{not_full p.repr}))
+  (ht:ht s)
+  (off: R.ref nat) (cont: R.ref bool)
+  (k:s.keyt) (v:s.valt)
+=
+  exists_ (fun (voff:nat) ->
+    exists_ (fun (vcont:bool) ->
+      insert_loop_inv_def b pht ht off cont k v voff vcont))
+
 // [@@expect_failure]
 ```pulse
 fn insert (#s:pht_sig) (#pht:(p:pht s{not_full p.repr})) 
@@ -39,36 +70,58 @@ fn insert (#s:pht_sig) (#pht:(p:pht s{not_full p.repr}))
   requires models s pht ht
   ensures  models s (PHT.insert pht k v) ht
 {
-  unfold (models s pht ht);
   let sz = ht.sz;
   let a = ht.contents;
   let cidx = canonical_index k sz;
   let mut off = coerce_nat 0;
   let mut cont = true;
+
+  // assume_ (exists_ (fun b -> insert_loop_inv b pht ht off cont k v));
+  // with b.
+  //   assert (insert_loop_inv b pht ht off cont k v);
+  // introduce
+  //   exists (b:bool). insert_loop_inv b pht ht off cont k v
+  //   with (0 <= ht.sz && = true);
+
+  // rewrite (models s pht ht)
+  //       as (models s (match true with | true -> pht | _ -> PHT.insert pht k v) ht);
+  // fold (insert_loop_inv_def true pht ht off cont k v 0 true);
+  // rewrite (insert_loop_inv_def true pht ht off cont k v 0 true)
+  //      as (insert_loop_inv_def true pht ht off cont k v (reveal (hide 0)) (reveal (hide true)));
+  // introduce exists (voff:nat) (vcont:bool).
+  //             insert_loop_inv_def true pht ht off cont k v (reveal voff) (reveal vcont)
+  //      with 0 true;
+  // assert emp;
+  // with (voff:Ghost.erased nat) (vcont:Ghost.erased bool).
+  //   assert (insert_loop_inv_def true pht ht off cont k v (Ghost.reveal voff) (Ghost.reveal vcont));
+
+  // assert (insert_loop_inv_def true pht ht off cont k v (Ghost.reveal voff) (Ghost.reveal vcont));
+  // rewrite (insert_loop_inv_def true pht ht off cont k v (Ghost.reveal voff) (Ghost.reveal vcont))
+  //      as (insert_loop_inv_def true pht ht off cont k v
+  //           (reveal (hide (reveal (hide (reveal voff)))))
+  //           (reveal (hide (reveal (hide (reveal vcont))))));
+
+  // rewrite (insert_loop_inv_def true pht ht off cont k v (reveal (hide voff)) (reveal (hide vcont)))
+  //      as (insert_loop_inv_def true pht ht off cont k v (reveal (hide voff)) (reveal (hide vcont)))
+  //fold (insert_loop_inv true pht ht off cont k v);
+    
+
+  // rewrite (exists (voff:nat) (vcont:bool).
+  //             insert_loop_inv_def true pht ht off cont k v (reveal voff) (reveal vcont))
+  //      as (insert_loop_inv true pht ht off cont k v);
+  assume_ (insert_loop_inv true pht ht off cont k v);
+
+  assert emp;
+
+  let zz = 42;
   while (let voff = !off; let vcont = !cont; (voff <= sz && vcont = true))
-  invariant b. exists (voff:nat) (vcont:bool) (s:Seq.lseq (cell s.keyt s.valt) pht.sz). (
-    A.pts_to ht.contents full_perm s `star`
-    // `@(if vcont=true 
-    //   then (A.pts_to ht.contents full_perm pht.repr) 
-    //   else (A.pts_to ht.contents full_perm (PHT.insert pht k v).repr)) `star`
-    R.pts_to off full_perm voff **
-    R.pts_to cont full_perm vcont **
-    pure (
-      pht.sz == ht.sz /\
-      voff >= 0 /\ voff <= sz /\
-      // walk_ pht.repr cidx k off == PHT.insert pht k v /\
-      // walk pht.repr cidx k off == lookup_repr pht.repr k /\
-      // strong_all_used_not_by #s #sz pht.repr cidx voff k /\
-      (if vcont=true
-        then s == pht.repr
-        else s == (PHT.insert pht k v).repr) /\
-      b == (voff <= sz && vcont = true)
-    )
-  )
+  invariant b. insert_loop_inv b pht ht off cont k v
   {
+    assume_ (exists_ (fun b -> insert_loop_inv b pht ht off cont k v));
     // if (off=sz) {
     // admit()
     // } else {
+      (*
     let voff = !off;
     let idx = coerce_us ((cidx+voff)%sz);
     assume_ (pure (US.v idx < pht.sz)); // FIXME: can prove based on modulo calc above
@@ -101,7 +154,10 @@ fn insert (#s:pht_sig) (#pht:(p:pht s{not_full p.repr}))
         cont := false;
         ()
       }
-    };};
+      *)
+      ()
+    //};
+    };
     fold (models s (PHT.insert pht k v) ht);
     ()
 }
